add basic introduction tactics

src/Iris/Proofmode/Classes.lean
@@ -11,8 +11,8 @@ class AsEmpValid2 (φ : Prop) {PROP : outParam Type} (P : outParam PROP) where
   [bi : BI PROP]
   as_emp_valid : φ ↔ ⊢ P
 
-instance [as : @AsEmpValid1 φ PROP P] : BI PROP := as.bi
-instance [as : @AsEmpValid2 φ PROP P] : BI PROP := as.bi
+instance [inst : @AsEmpValid1 φ PROP P] : BI PROP := inst.bi
+instance [inst : @AsEmpValid2 φ PROP P] : BI PROP := inst.bi
 
 class AsEmpValid (φ : Prop) {PROP : Type} (P : PROP) extends
   AsEmpValid1 φ P,
@@ -20,5 +20,19 @@ class AsEmpValid (φ : Prop) {PROP : Type} (P : PROP) extends
 
 theorem as_emp_valid_1 [BI PROP] (P : PROP) [AsEmpValid1 φ P] : φ → ⊢ P := sorry
 theorem as_emp_valid_2 (φ : Prop) [AsEmpValid2 φ P] : (⊢ P) → φ := sorry
+
+
+class FromImpl [BI PROP] (P : PROP) (Q1 Q2 : outParam PROP) where
+  from_impl : (Q1 → Q2) ⊢ P
+
+class FromWand [BI PROP] (P : PROP) (Q1 Q2 : outParam PROP) where
+  from_wand : (Q1 -∗ Q2) ⊢ P
+
+
+class IntoPersistent (p : Bool) [BI PROP] (P : PROP) (Q : outParam PROP) where
+  into_persistent : <pers>?p P ⊢ <pers> Q
+
+class FromAffinely [BI PROP] (P : outParam PROP) (Q : PROP) where
+  from_affinely : <affine> Q ⊢ P
 
 end Iris.Proofmode
