src/Iris/Proofmode/Instances.lean
@@ -17,4 +17,71 @@ instance as_emp_valid_equiv (P Q : PROP) : AsEmpValid (P ≡ Q) `[iprop| P ∗-�
   bi := bi
   as_emp_valid := sorry
 
+-- FromImpl
+instance from_impl_impl (P1 P2 : PROP) :
+  FromImpl `[iprop| P1 → P2] P1 P2
+where
+  from_impl := sorry
+
+-- FromWand
+instance from_wand_wand (P1 P2 : PROP) :
+  FromWand `[iprop| P1 -∗ P2] P1 P2
+where
+  from_wand := sorry
+
+-- IntoPersistent
+@[instance 30]
+instance into_persistent_persistently (p : Bool) (P Q : PROP) :
+  [IntoPersistent true P Q] →             -- if <pers> P ⊢ <pers> Q
+  IntoPersistent p `[iprop| <pers> P] Q   -- then <pers>?p <pers> P ⊢ <pers> Q
+where
+  into_persistent := sorry
+
+@[instance 30]
+instance into_persistent_affinely (p : Bool) (P Q : PROP) :
+  [IntoPersistent p P Q] →                -- if <pers>?p P ⊢ <pers> Q
+  IntoPersistent p `[iprop| <affine> P] Q -- then <pers>?p <affine> P ⊢ <pers> Q
+where
+  into_persistent := sorry
+
+@[instance 30]
+instance into_persistent_intuitionistically (p : Bool) (P Q : PROP) :
+  [IntoPersistent true P Q] →             -- if <pers> P ⊢ <pers> Q
+  IntoPersistent p `[iprop| □ P] Q        -- then <pers>?p □ P ⊢ <pers> Q
+where
+  into_persistent := sorry
+
+@[instance 20]
+instance into_persistent_here (P : PROP) :
+  IntoPersistent true P P                 -- always <pers> P ⊢ <pers> P
+where
+  into_persistent := sorry
+
+@[instance 10]
+instance into_persistent_persistent (P : PROP) :
+  [Persistent P] →                        -- if P is persistent
+  IntoPersistent false P P                -- then P ⊢ <pers> P
+where
+  into_persistent := sorry
+
+-- FromAffinely
+@[instance 20]
+instance from_affinely_affine (P : PROP) :
+  [Affine P] →                                  -- if P is affine
+  FromAffinely P P                              -- then <affine> P ⊢ P
+where
+  from_affinely := sorry
+
+@[instance 10]
+instance from_affinely_default (P : PROP) :
+  FromAffinely `[iprop| <affine> P] P           -- always <affine> P ⊢ <affine> P
+where
+  from_affinely := sorry
+
+@[instance 10]
+instance from_affinely_intuitionistically (P : PROP) :
+  FromAffinely `[iprop| □ P] `[iprop| <pers> P] -- always <affine> <pers> P ⊢ □ P
+where
+  from_affinely := sorry
+
 end Iris.Proofmode
