src/Iris/Proofmode/Tactics.lean
@@ -23,10 +23,11 @@ elab "iStartProof" : tactic => do
     return ()
 
   -- create environment
-  evalTactic (← `(tactic|
+  try evalTactic (← `(tactic|
     refine (as_emp_valid_2 _ ?_) ;
     refine (tac_start _ ?_)
   ))
+  catch _ => throwError "unable to start proof mode"
 
 
 elab "iStopProof" : tactic => do
@@ -39,10 +40,11 @@ elab "iStopProof" : tactic => do
   if !(isEnvsEntails expr) then
     throwError "not in proof mode"
 
-  evalTactic (← `(tactic|
+  try evalTactic (← `(tactic|
     simp only [envs_entails, of_envs] ;
     pmReduce
   ))
+  catch _ => throwError "unable to stop proof mode"
 
 
 namespace Internal
@@ -58,6 +60,8 @@ scoped elab "iRename " categ:(&"p" <|> &"s") idx:num name:ident : tactic => do
   let some idx := idx.getAtomValFromNode? `num String.toNat?
     | throwUnsupportedSyntax
   let name := name.getId
+  if name.isAnonymous then
+    throwUnsupportedSyntax
 
   -- parse goal
   let goal :: _ ← getUnsolvedGoals
@@ -94,5 +98,76 @@ scoped elab "iRename " categ:(&"p" <|> &"s") idx:num name:ident : tactic => do
   setMVarType goal expr
 
 end Internal
+
+
+private def extractEnvsEntailsFromGoal? (startProofMode : Bool := false) : TacticM <| Expr × Expr × Expr := do
+  if startProofMode then
+    evalTactic (← `(tactic|
+      iStartProof
+    ))
+
+  let goal :: _ ← getUnsolvedGoals
+    | throwNoGoalsToBeSolved
+  let expr ← (← getMVarType goal) |> instantiateMVars
+
+  let some envsEntails := extractEnvsEntails? expr
+    | throwError "not in proof mode"
+
+  return envsEntails
+
+
+elab "iIntro " colGt name:ident : tactic => do
+  -- parse syntax
+  if name.getId.isAnonymous then
+    throwUnsupportedSyntax
+
+  -- extract environment
+  let (_, Γₛ, _) ← extractEnvsEntailsFromGoal? true
+
+  -- determine hypothesis list length
+  let some s_length := Γₛ.asListExpr_length?
+    | throwError "ill-formed proof environment"
+
+  -- introduce hypothesis
+  try evalTactic (← `(tactic|
+    first
+    | refine tac_impl_intro _ ?_
+    | refine tac_wand_intro _ ?_
+    | fail
+  ))
+  catch _ => throwError "failed to introduce hypothesis"
+
+  -- normalize `envs_entails` and name hypothesis
+  evalTactic (← `(tactic|
+    pmReduce ;
+    iRename s $(quote s_length) $name
+  ))
+
+elab "iIntro " colGt "#" colGt name:ident : tactic => do
+  -- parse syntax
+  if name.getId.isAnonymous then
+    throwUnsupportedSyntax
+
+  -- extract environment
+  let (Γₚ, _, _) ← extractEnvsEntailsFromGoal? true
+
+  -- determine hypothesis list length
+  let some p_length := Γₚ.asListExpr_length?
+    | throwError "ill-formed proof environment"
+
+  -- introduce hypothesis
+  try evalTactic (← `(tactic|
+    first
+    | refine tac_impl_intro_intuitionistic _ ?_
+    | refine tac_wand_intro_intuitionistic _ ?_
+    | fail
+  ))
+  catch _ => throwError "failed to introduce hypothesis"
+
+  -- normalize `envs_entails` and name hypothesis
+  evalTactic (← `(tactic|
+    pmReduce ;
+    iRename p $(quote p_length) $name
+  ))
 
 end Iris.Proofmode
