src/Iris/Proofmode/Theorems.lean
@@ -1,13 +1,48 @@
 import Iris.BI
 import Iris.Proofmode.Classes
 import Iris.Proofmode.Environments
+import Iris.Std.List
+import Iris.Std.TC
 
 namespace Iris.Proofmode
-open Iris.BI
+open Iris.BI Iris.Std
 
 variable [BI PROP]
 
 -- proof mode
-theorem tac_start (P : PROP) : envs_entails ⟨[], []⟩ P → ⊢ P := sorry
+theorem tac_start (P : PROP) :
+  envs_entails ⟨[], []⟩ P →
+  ⊢ P
+:= sorry
+
+-- implication and wand
+theorem tac_impl_intro {Γₚ Γₛ : List PROP} {P Q : PROP} (R : PROP) :
+  [FromImpl R P Q] →
+  [TCIte Γₛ.isEmptyR TCTrue (Persistent P)] →
+  [FromAffinely P' P] →
+  envs_entails ⟨Γₚ, Γₛ.concat P'⟩ Q →
+  envs_entails ⟨Γₚ, Γₛ⟩ R
+:= sorry
+
+theorem tac_impl_intro_intuitionistic {Γₚ Γₛ : List PROP} {P P' Q : PROP} (R : PROP) :
+  [FromImpl R P Q] →
+  [IntoPersistent false P P'] →
+  envs_entails ⟨Γₚ.concat P', Γₛ⟩ Q →
+  envs_entails ⟨Γₚ, Γₛ⟩ R
+:= sorry
+
+theorem tac_wand_intro {Γₚ Γₛ : List PROP} {P Q : PROP} (R : PROP) :
+  [FromWand R P Q] →
+  envs_entails ⟨Γₚ, Γₛ.concat P⟩ Q →
+  envs_entails ⟨Γₚ, Γₛ⟩ R
+:= sorry
+
+theorem tac_wand_intro_intuitionistic {Γₚ Γₛ : List PROP} {P P' Q : PROP} (R : PROP) :
+  [FromWand R P Q] →
+  [IntoPersistent false P P'] →
+  [TCOr (Affine P) (Absorbing Q)] →
+  envs_entails ⟨Γₚ.concat P', Γₛ⟩ Q →
+  envs_entails ⟨Γₚ, Γₛ⟩ R
+:= sorry
 
 end Iris.Proofmode
