src/Iris/Std.lean
@@ -2,3 +2,4 @@ import Iris.Std.Classes
 import Iris.Std.Expr
 import Iris.Std.List
 import Iris.Std.Syntax
+import Iris.Std.TC
