src/Iris/Std/TC.lean
@@ -1,0 +1,30 @@
+namespace Iris.Std
+
+set_option checkBinderAnnotations false
+
+class inductive TCFalse
+
+
+class inductive TCTrue
+  | t
+
+instance : TCTrue := TCTrue.t
+
+
+class inductive TCOr (T U : Sort _)
+  | l : [T] → TCOr T U
+  | r : [U] → TCOr T U
+
+instance [t : T] : TCOr T U := @TCOr.l T U t
+instance [u : U] : TCOr T U := @TCOr.r T U u
+
+
+/-- Type class instances search requires `c` to be fully reduced. -/
+class inductive TCIte (c : Bool) (T U : Sort _)
+  | t : (_ : c = true) → [T] → TCIte c T U
+  | e : (_ : c = false) → [U] → TCIte c T U
+
+instance [t : T] : TCIte true T U := @TCIte.t true T U (by rfl) t
+instance [u : U] : TCIte false T U := @TCIte.e false T U (by rfl) u
+
+end Iris.Std
